\documentclass{beamer}
\usetheme{ucl}

\input{package}
\input{macro}


\setbeamersize{description width=2em}
%%% Remove nav symbols (and shift any logo down to corner)
\setbeamertemplate{navigation symbols}{\vspace{-2ex}}
\setbeamertemplate{footline}[author title date]
\setbeamercolor{banner}{bg=darkpurple}
\useinnertheme{blockborder}

\graphicspath{{./images/} }
\title[Translations between bases in B-eS]{Translations between bases in Base-extension Semantics}
%\author{\texorpdfstring{Yll Buzoku\newline\url{y.buzoku@ucl.ac.uk}}{https://www.homepages.ucl.ac.uk/~zcapybu/}}
\author{Yll Buzoku}
\institute[UCL]{%
  Department of Computer Science \\ %
  University College London
}
\date{November 22, 2024}

\AtBeginSection[]
{
  \begin{frame}
    \frametitle{Presentation root directory}
    \tableofcontents[currentsection]
  \end{frame}
}

\begin{document}
%%%%%%%%%%%%%%%%%%%%%%%%%%%%%%%%%%%%%%%%%%%%%%%%%%%%%%%%
%%%%%%%%%%%%%%%%%%%%%%%%%%%%%%%%%%%%%%%%%%%%%%%%%%%%%%%%
\begin{frame}
\titlepage
\end{frame}
%%%%%%%%%%%%%%%%%%%%%%%%%%%%%%%%%%%%%%%%%%%%%%%%%%%%%%%%
%%%%%%%%%%%%%%%%%%%%%%%%%%%%%%%%%%%%%%%%%%%%%%%%%%%%%%%%
\section*{Goals for this presentation}
\begin{frame}{Goals for this talk}
\begin{itemize}
\item Introduce the concept of bases and general inference figures
\item Introduce two notions of atomic derivability
\item Show how one may relate these notions of atomic derivability
\end{itemize}
\end{frame}
%%%%%%%%%%%%%%%%%%%%%%%%%%%%%%%%%%%%%%%%%%%%%%%%%%%%%%%%
%%%%%%%%%%%%%%%%%%%%%%%%%%%%%%%%%%%%%%%%%%%%%%%%%%%%%%%%
\begin{frame}{Presentation root directory}
\tableofcontents
\end{frame}
%%%%%%%%%%%%%%%%%%%%%%%%%%%%%%%%%%%%%%%%%%%%%%%%%%%%%%%%
%%%%%%%%%%%%%%%%%%%%%%%%%%%%%%%%%%%%%%%%%%%%%%%%%%%%%%%%
\section{Bases and inference figures}
\begin{frame}{Notation}
	\begin{itemize}%[label={-}]
		\item $\At$ represents a fixed, countably infinite set of propositional atoms. 
		\item Lower case latin letters represent propositional atoms.
		\item Upper case latin letters represent finite multisets of propositional atoms. 
		\item Atomic multiset is taken to mean multiset of propositional atoms.
		\item The sum of two multisets $\at{P}$ and $\at{Q}$ is denoted $\at{P}\msetsum\at{Q}$. 
	\end{itemize}
\end{frame}
%%%%%%%%%%%%%%%%%%%%%%%%%%%%%%%%%%%%%%%%%%%%%%%%%%%%%%%%
\begin{frame}{Atomic rules}
Atomic rules take the form: \newline 
\begin{center}
	$\langle\langle P_1,p_1\rangle,\dots,\langle P_n,p_n\rangle,p\rangle$	
\end{center}
\end{frame}
%%%%%%%%%%%%%%%%%%%%%%%%%%%%%%%%%%%%%%%%%%%%%%%%%%%%%%%%
\begin{frame}{Atomic rules}
Pictorially, we can represent this as: \newline 
\begin{center}
	\begin{prooftree}
		\AxiomC{$[P_1]$}
		\noLine
		\UnaryInfC{$p_1$}
		\AxiomC{$\dots$}
		\AxiomC{$[P_n]$}
		\noLine
		\UnaryInfC{$p_n$}
		\TrinaryInfC{$p$}
	\end{prooftree}
	\pause
	\vspace{1.8cm}
	\emph{Any idea what these figures are supposed to look like?}\newline
	\pause
	\textbf{Natural deduction!}
\end{center}
\end{frame}
%%%%%%%%%%%%%%%%%%%%%%%%%%%%%%%%%%%%%%%%%%%%%%%%%%%%%%%%
\begin{frame}{Contextual atomic rules}
	Contextual atomic rules are rules which may have contextual brackets distributed across them.
\end{frame}
%%%%%%%%%%%%%%%%%%%%%%%%%%%%%%%%%%%%%%%%%%%%%%%%%%%%%%%%
\begin{frame}{Contextual atomic rules}
Pictorially, we can represent such rules as: \newline 

\begin{prooftree}
	\AxiomC{$\left\{\raisebox{-0.5em}{$\deduce{p_{1_1} \quad \ldots \quad p_{1_{l_1}}}{[P_{1_1}] \hspace{2.8em} [P_{1_{l_n}}]}$}\right\}$}
	\AxiomC{$\ldots$}
	\AxiomC{$\left\{\raisebox{-0.5em}{$\deduce{p_{n_1} \quad \ldots \quad p_{n_{l_n}}}{[P_{n_1}] \hspace{2.8em} [P_{n_{l_n}}]}$}\right\}$}
	\TrinaryInfC{$p$}
\end{prooftree}
\pause
or linearly, like this:\newline
\begin{center}
	$\langle\openaddrule \langle P_{1_i},p_{1_i}\rangle\closeaddrule^{l_1}_{i=1}, \dots, \openaddrule \langle P_{n_i},p_{n_i}\rangle\closeaddrule^{l_n}_{i=1}, p\rangle$
\end{center}
\end{frame}
%%%%%%%%%%%%%%%%%%%%%%%%%%%%%%%%%%%%%%%%%%%%%%%%%%%%%%%%
\begin{frame}{Examples of atomic rules}
	\begin{itemize}
		\item $\langle\openaddrule\langle \emptymultiset, a\rangle\closeaddrule, c\rangle$
		\item $\langle\openaddrule\langle \emptymultiset,a\rangle\closeaddrule, \openaddrule\langle c,d,e\rangle, \langle f,g\rangle\closeaddrule, q\rangle$ 
		\item $\langle\openaddrule\langle a, b\rangle\closeaddrule, \openaddrule\langle \emptymultiset,e\rangle\closeaddrule, \langle f,g\rangle, q\rangle$
	\end{itemize}
	\vspace{0.5cm}
	\begin{itemize}
		\item $\langle\langle \emptymultiset,a\rangle,c\rangle$
		\item $\langle\langle \emptymultiset,b\rangle,c\rangle$
		\item $\langle\langle \emptymultiset,c\rangle,\langle a,p\rangle, \langle b,p\rangle, p\rangle$
	\end{itemize}
\end{frame}
%%%%%%%%%%%%%%%%%%%%%%%%%%%%%%%%%%%%%%%%%%%%%%%%%%%%%%%%
\begin{frame}{Bases}
	\begin{definition}[Base]
		A base is a set of atomic rules.\newline
		\pause
		A base is said to be contextual if it contains contextual rules.\\
		Else it is said to be context-free.
	\end{definition}
	\pause
	\begin{itemize}
		\item $\{(\openaddrule\Rightarrow a\closeaddrule\Rightarrow c), (\openaddrule a\Rightarrow c\closeaddrule\Rightarrow b)\}$
		%
		\item $\{(\openaddrule \Rightarrow a\closeaddrule\Rightarrow c), (\openaddrule a\Rightarrow c\closeaddrule\Rightarrow b),(\openaddrule\Rightarrow a\closeaddrule,\openaddrule\Rightarrow a\closeaddrule\Rightarrow a)\}$
		%
		\item $\{(\openaddrule \Rightarrow a\closeaddrule\Rightarrow c), (\openaddrule a\Rightarrow c\closeaddrule\Rightarrow b),(\openaddrule\Rightarrow d\closeaddrule,\openaddrule\Rightarrow d\closeaddrule\Rightarrow a),(\openaddrule\Rightarrow a\closeaddrule\Rightarrow d)\}$
	\end{itemize}
\end{frame}
%%%%%%%%%%%%%%%%%%%%%%%%%%%%%%%%%%%%%%%%%%%%%%%%%%%%%%%%
%%%%%%%%%%%%%%%%%%%%%%%%%%%%%%%%%%%%%%%%%%%%%%%%%%%%%%%%
\section{Atomic derivability}
\begin{frame}{Atomic derivability}
\begin{definition}[Context-free atomic derivability $\deriveBaseIPL{\baseB}$]
The relation of derivability in a context-free base $\baseB$, is defined as so:
\begin{itemize}
    \item[Ref] $S\deriveBaseIPL{\baseB}p$ if $p\in S$.
    \item[App] For $\langle\langle P_1, p_1\rangle, \dots, \langle P_n, p_n\rangle, q\rangle \in \baseB$ and $S\msetsum P_i\deriveBaseIPL{\baseB}p_i$ for each $i\in \{1,\dots,n\}$ then $S\deriveBaseIPL{\baseB}q$.
\end{itemize}
\end{definition}
\pause
\begin{definition}[Contextual atomic derivability $\deriveBaseM{\baseB}$]
The relation of derivability in a contextual base $\baseB$, is defined as so:
\begin{itemize}
    \item[Ref] $p\deriveBaseM{\baseB}p$.
    \item[App] For $\langle\openaddrule\langle P_{1_i}, p_{1_{i}}\rangle\Closeaddrule{i=1}{l_1},\dots,\openaddrule \langle P_{n_i}, p_{n_{i}}\rangle \Closeaddrule{i=1}{l_n}, q\rangle \in \baseB$ and $C_i\msetsum P_{i_j}\deriveBaseM{\baseB}p_{i_j}$ for each $i\in \{1,\dots,n\}$ and $j \in \{1,\dots,l_i\}$ then $C_1\msetsum\dots\msetsum C_n\deriveBaseM{\baseB}q$.
\end{itemize}
\end{definition}

\end{frame}
%%%%%%%%%%%%%%%%%%%%%%%%%%%%%%%%%%%%%%%%%%%%%%%%%%%%%%%%
\begin{frame}{Example derivations}
	\begin{example}[Derivation terminations]
		Let $\baseB=\{(\Rightarrow a), (\openaddrule \Rightarrow a \closeaddrule,\openaddrule\Rightarrow b\closeaddrule\Rightarrow c)\}$
		\begin{prooftree}
			\AxiomC{}
			\RightLabel{Ref}
			\UnaryInfC{$b\deriveBaseM{\baseB}b$}
			\AxiomC{}
			\RightLabel{$\Rightarrow a$}
			\UnaryInfC{$\deriveBaseM{\baseB}a$}
			\RightLabel{$\openaddrule \Rightarrow a \closeaddrule,\openaddrule\Rightarrow b\closeaddrule\Rightarrow c$}
			\BinaryInfC{$b\deriveBaseM{\baseB}c$}
		\end{prooftree}
		Therefore, in $\baseB$, the atom $c$ is derivable from $b$. 
	\end{example}
\end{frame}
%%%%%%%%%%%%%%%%%%%%%%%%%%%%%%%%%%%%%%%%%%%%%%%%%%%%%%%%
\begin{frame}{Example derivations}
	\begin{example}[Invalid derivation]
		By the definition of $\deriveBaseM{\baseB}$, deriving $a$ from $a\msetsum a$ in the empty base is not possible, i.e. $a\msetsum a\deriveBaseM{\emptybase}a$ is not possible.
	\end{example}
	\pause
	\begin{example}[Invalid derivation 2]
		Let $\baseB=\{(\openaddrule\Rightarrow a\closeaddrule\Rightarrow c), (\openaddrule a\Rightarrow c\closeaddrule\Rightarrow b)\}$
		\begin{prooftree}
			\AxiomC{$\times$}
			\UnaryInfC{$a\msetsum a\deriveBaseM{\baseB}a$}
			\RightLabel{$\openaddrule\Rightarrow a\closeaddrule\Rightarrow c$}
			\UnaryInfC{$a\msetsum a\deriveBaseM{\baseB}c$}
			\RightLabel{$\openaddrule a\Rightarrow c\closeaddrule\Rightarrow b$}
			\UnaryInfC{$a\deriveBaseM{\baseB}b$}
		\end{prooftree}
		We see that in this base, $a$ is not derivable from $a\msetsum a$.
	\end{example}
\end{frame}
%%%%%%%%%%%%%%%%%%%%%%%%%%%%%%%%%%%%%%%%%%%%%%%%%%%%%%%%
\begin{frame}{Example derivations}
	\begin{example}[A possible fix for invalid derivation 2]
		Let $\baseC=\{(\openaddrule \Rightarrow a\closeaddrule\Rightarrow c), (\openaddrule a\Rightarrow c\closeaddrule\Rightarrow b),(\openaddrule\Rightarrow a\closeaddrule,\openaddrule\Rightarrow a\closeaddrule\Rightarrow a)\}$
		\begin{prooftree}
			\AxiomC{}
			\RightLabel{Ref}
			\UnaryInfC{$a\deriveBaseM{\baseC}a$}			
			\AxiomC{}
			\RightLabel{Ref}
			\UnaryInfC{$a\deriveBaseM{\baseC}a$}
			\RightLabel{$\openaddrule\Rightarrow a\closeaddrule,\openaddrule\Rightarrow a\closeaddrule\Rightarrow a$}
			\BinaryInfC{$a\msetsum a\deriveBaseM{\baseC}a$}
			\RightLabel{$\openaddrule \Rightarrow a\closeaddrule\Rightarrow c$}
			\UnaryInfC{$a\msetsum a\deriveBaseM{\baseC}c$}
			\RightLabel{$\openaddrule a\Rightarrow c\closeaddrule\Rightarrow b$}
			\UnaryInfC{$a\deriveBaseM{\baseC}b$}
		\end{prooftree}
		Note that $\baseC\supset\baseB$\hspace{5pt}!!
	\end{example}
\end{frame}
%%%%%%%%%%%%%%%%%%%%%%%%%%%%%%%%%%%%%%%%%%%%%%%%%%%%%%%%
\begin{frame}{Example derivations}
	\begin{example}[Another possible fix for invalid derivation 2]
		Let $\baseD=\{(\openaddrule \Rightarrow a\closeaddrule\Rightarrow c), (\openaddrule a\Rightarrow c\closeaddrule\Rightarrow b),(\openaddrule\Rightarrow d\closeaddrule,\openaddrule\Rightarrow d\closeaddrule\Rightarrow a),(\openaddrule\Rightarrow a\closeaddrule\Rightarrow d)\}$
		\begin{prooftree}
			\AxiomC{}
			\RightLabel{Ref}
			\UnaryInfC{$a\deriveBaseM{\baseD}a$}
			\RightLabel{$\openaddrule\Rightarrow a\closeaddrule\Rightarrow d$}
			\UnaryInfC{$a\deriveBaseM{\baseD}d$}
			\AxiomC{}
			\RightLabel{Ref}
			\UnaryInfC{$a\deriveBaseM{\baseD}a$}			
			\RightLabel{$\openaddrule\Rightarrow a\closeaddrule\Rightarrow d$}
			\UnaryInfC{$a\deriveBaseM{\baseD}d$}
			\RightLabel{$\openaddrule\Rightarrow d\closeaddrule,\openaddrule\Rightarrow d\closeaddrule\Rightarrow a$}
			\BinaryInfC{$a\msetsum a\deriveBaseM{\baseD}a$}
			\RightLabel{$\openaddrule \Rightarrow a\closeaddrule\Rightarrow c$}
			\UnaryInfC{$a\msetsum a\deriveBaseM{\baseD}c$}
			\RightLabel{$\openaddrule a\Rightarrow c\closeaddrule\Rightarrow b$}
			\UnaryInfC{$a\deriveBaseM{\baseD}b$}
		\end{prooftree}
	\end{example}
\end{frame}
%%%%%%%%%%%%%%%%%%%%%%%%%%%%%%%%%%%%%%%%%%%%%%%%%%%%%%%%
\begin{frame}{Example derivations}
	\begin{example}[A live complicated derivation!]
		Consider a base $\baseB$ with only the following rules:
		\begin{itemize}
			\item $\openaddrule\Rightarrow c\closeaddrule,\openaddrule\Rightarrow y\closeaddrule\Rightarrow f$
			\item $\Rightarrow z$
			\item $\openaddrule \Rightarrow a\closeaddrule,\openaddrule \Rightarrow b\closeaddrule,\openaddrule\Rightarrow z\closeaddrule\Rightarrow h$
			\item $\openaddrule\Rightarrow h\closeaddrule\Rightarrow g$
			\item $\openaddrule\Rightarrow x\closeaddrule,\openaddrule\Rightarrow g\closeaddrule\Rightarrow e$
			\item $\openaddrule x\Rightarrow e\closeaddrule,\openaddrule y\Rightarrow f\closeaddrule\Rightarrow d$
		\end{itemize}
		is there a derivation of $d$ from the multiset $a\msetsum b\msetsum c$ in $\baseB$?
%		\begin{prooftree}
%			\AxiomC{}
%			\RightLabel{Ref}
%			\UnaryInfC{$f\deriveBaseM{\baseB}f$}
%			\AxiomC{}
%			\RightLabel{Ref}
%			\UnaryInfC{$c\deriveBaseM{\baseB}c$}
%			\RightLabel{$\openaddrule\Rightarrow c\closeaddrule,\openaddrule\Rightarrow y\closeaddrule\Rightarrow f$}
%			\BinaryInfC{$c,y\deriveBaseM{\baseB}f$}
%			\AxiomC{}
%			\RightLabel{$\Rightarrow z$}
%			\UnaryInfC{$\deriveBaseM{\baseB}z$}
%			\AxiomC{}
%			\RightLabel{Inf}
%			\UnaryInfC{$b\deriveBaseM{\baseB}b$}
%			\AxiomC{}
%			\RightLabel{Inf}
%			\UnaryInfC{$a\deriveBaseM{\baseB}a$}
%			\RightLabel{$\openaddrule \Rightarrow a\closeaddrule,\openaddrule \Rightarrow b\closeaddrule,\openaddrule\Rightarrow z\closeaddrule\Rightarrow h$}
%			\TrinaryInfC{$a,b,\deriveBaseM{\baseB}h$}
%			\RightLabel{$\openaddrule\Rightarrow h\closeaddrule\Rightarrow g$}
%			\UnaryInfC{$a,b\deriveBaseM{\baseB}g$}
%			\AxiomC{}
%			\RightLabel{Ref}
%			\UnaryInfC{$x\deriveBaseM{\baseB}x$}
%			\RightLabel{$\openaddrule\Rightarrow x\closeaddrule,\openaddrule\Rightarrow g\closeaddrule\Rightarrow e$}
%			\BinaryInfC{$a,b,x\deriveBaseM{\baseB}e$}
%			\RightLabel{$\openaddrule x\Rightarrow e\closeaddrule,\openaddrule y\Rightarrow f\closeaddrule\Rightarrow d$}
%			\BinaryInfC{$a,b,c\deriveBaseM{\baseB}b$}
%		\end{prooftree}
	\end{example}
	\pause 
	\emph{Disclaimer: The fact I couldn't fit this derivation on the slide has nothing to do with why we are doing this derivation live :-)}
\end{frame}
%%%%%%%%%%%%%%%%%%%%%%%%%%%%%%%%%%%%%%%%%%%%%%%%%%%%%%%%
\begin{frame}{Example derivations}
	\begin{example}[A very interesting derivation]
		Let $\baseB = \{
		(\openaddrule\Rightarrow b\closeaddrule\Rightarrow c),
		(\openaddrule\Rightarrow a\closeaddrule,\openaddrule b\Rightarrow c\closeaddrule\Rightarrow d),
		(\openaddrule\Rightarrow d, \Rightarrow a \closeaddrule\Rightarrow e),
		(\openaddrule a\Rightarrow e\closeaddrule\Rightarrow f)
		\}$
		\begin{prooftree}
			\AxiomC{}
			\RightLabel{Ref}
			\UnaryInfC{$a\deriveBaseM{\baseB}a$}			
			\AxiomC{}
			\RightLabel{Ref}
			\UnaryInfC{$b\deriveBaseM{\baseB}b$}
			\RightLabel{$\openaddrule\Rightarrow b\closeaddrule\Rightarrow c$}
			\UnaryInfC{$b\deriveBaseM{\baseB}c$}
			\RightLabel{$\openaddrule\Rightarrow a\closeaddrule,\openaddrule b\Rightarrow c\closeaddrule\Rightarrow d$}
			\BinaryInfC{$a\deriveBaseM{\baseB}d$}
			\AxiomC{}
			\RightLabel{Ref}
			\UnaryInfC{$a\deriveBaseM{\baseB}a$}
			\RightLabel{$\openaddrule\Rightarrow d, \Rightarrow a \closeaddrule\Rightarrow e$}
			\BinaryInfC{$a\deriveBaseM{\baseB}e$}
			\RightLabel{$\openaddrule a\Rightarrow e\closeaddrule\Rightarrow f$}
			\UnaryInfC{$\deriveBaseM{\baseB}f$}
		\end{prooftree}
	\end{example}
\end{frame}
%%%%%%%%%%%%%%%%%%%%%%%%%%%%%%%%%%%%%%%%%%%%%%%%%%%%%%%%
%%%%%%%%%%%%%%%%%%%%%%%%%%%%%%%%%%%%%%%%%%%%%%%%%%%%%%%%
\section{Comparing relations}
\begin{frame}{Comparing relations}

\end{frame}
%%%%%%%%%%%%%%%%%%%%%%%%%%%%%%%%%%%%%%%%%%%%%%%%%%%%%%%%
\begin{frame}{Thank you!}
\begin{figure}
	\begin{center}
	  \includegraphics[width=\textwidth]{dosthanks2.png}
	  \caption{Thank you from DOS!\,:D}
	\end{center}
  \end{figure}
\end{frame}
%%%%%%%%%%%%%%%%%%%%%%%%%%%%%%%%%%%%%%%%%%%%%%%%%%%%%%%%
\begin{frame}[allowframebreaks]
	\frametitle{References}
	\nocite{*}
	\bibliographystyle{amsalpha}
	\bibliography{./refs/refs.bib}
\end{frame}
%%%%%%%%%%%%%%%%%%%%%%%%%%%%%%%%%%%%%%%%%%%%%%%%%%%%%%%%
\end{document}
